\subsection{Normal Forms}\label{subsec:normal-forms}
\subsubsection{Chomsky Normal Form}\label{subsubsec:chomsky-normal-form}
\begin{definition}
    A context-free language \(G\) is in \textbf{Chomsky Normal Form}\footnote{This is also called \textbf{Chomsky Reduced Form}. Sometimes, Chomsky Normal Form includes the production \(S\to\varepsilon \). In our usage, CNF and CRF are identical and do not include a \(\varepsilon \) production.}if all of its productions are of the form 
    \begin{align*}A &\to BC\\
                  A &\to a\\
    \end{align*}
\end{definition}

\begin{theorem}
    If \(G\) is a context-free grammar, there exists a Chomsky Normal Form grammar for \(L(G)-\{\varepsilon \} \)
\end{theorem}

\begin{proof}

\end{proof}

To convert to Chomsky Normal Form, first preprocess the CFG\@. Then, for any production containing a non-solitary terminal, \(a\), replace \(a\) with \(X_a\), where \(X_a\to a\). After this, we replace every production \[A\to X_1X_2\hdots X_n\] with the following productions

\begin{align*}
    A &\to X_1 A_1 \\
    A_1 &\to X_2 A_2 \\
    A_2 &\to X_3 A_3 \\
        &\vdots \\
    A_{n-2} &\to X_{n-1} X_n
\end{align*}

\subsubsection{Greibach Normal Form}\label{subsubsec:greibach-normal-form}
\begin{definition}
    A context-free language is in \textbf{Greibach Normal Form}\footnote{Sometimes, the production \(S\to\varepsilon \) is incuded. In our use, there is no \(\varepsilon \) production.} if all of its productions are of the form
    \[A\to aA_1A_2\hdots A_n\]
\end{definition}

To convert a CFG to Greibach Normal Form, you must remove left-recursion. First, preprocess the CFG\@. We can remove any \textit{direct recursion} of the form 

\[A\to A\alpha_1 \mid A\alpha_2 \mid A\alpha_3 \mid \hdots \mid A\alpha_m \mid \beta_1 \mid \beta_2 \mid \beta_3 \mid \hdots \mid \beta_n\] 

where no \(\beta_i\) begins with \(A\), by replacing the productions for \(A\) with 

\begin{align*}
    A  &\to \beta_1\mid \beta_2\mid \beta_3\mid \hdots \mid \beta_n\mid\beta_1 A'\mid \beta_2 A'\mid \beta_3 A'\mid \hdots \mid \beta_n A'\\
    A' &\to \alpha_1\mid \alpha_2\mid \alpha_3\mid \hdots \mid \alpha_m\mid \alpha_1 A'\mid \alpha_2 A'\mid \alpha_3 A' \mid \hdots \mid \alpha_m A'
\end{align*}

More generally, we eliminate \textit{indirect recursion} by ordering the non-terminals and performing the following algorithm:

\begin{algorithm}[H]
    \renewcommand{\thealgorithm}{}
    \caption{Returns CFG with left-recursion removed}\label{remove-left-recursion}
    \begin{algorithmic}[1]
    \Procedure{S}{G}
        \For{each non-terminal \(A_i\)}
            \For{each production \(A_i\to\alpha_i\)}
                \If{\(\alpha_i\) begins with \(A_j\) for \(j<i\)}
                    \State{let \(\beta_i\) be \(\alpha_i\) without the leading \(A_j\)}
                    \State{remove the production \(A_i\to\alpha_i\)}
                    \For{each production \(A_j\to\alpha_j\)}
                        \State{Add rule \(A_i\to\alpha_j \beta_i\)}
                    \EndFor{}
                \EndIf{}
            \EndFor{}
            \State{remove direct left recursion for \(A_i\)}
        \EndFor{}
    \EndProcedure{}
    \end{algorithmic}
    \end{algorithm}

Consider the following example:

\begin{align*}
    S &\to AS\mid a\\
    A &\to BS\mid b\\
    B &\to CS\mid c\\
    C &\to SS\mid d
\end{align*}

There is no preprocessing to do, since there are no useless or nullable variables and no unit productions. Notice that \(C\) includes indirect left-recursion. Thus, we write 

\begin{align*}
    C &\to ASS\mid aS\mid d\\
      &\to BSSS\mid bSS \mid aS\mid d\\
      &\to CSSSS\mid cSSS\mid bSS\mid aS\mid d
\end{align*}

Now, we eliminate the direct left-recursion from \(C\)

\begin{align*}
    C &\to cSSS\mid bSS\mid aS\mid d\mid cSSSC'\mid bSSC'\mid aSC'\mid dC'\\
    C' &\to SSSS\mid SSSSC'
\end{align*}

Next, we substitute the productions for \(C\) into \(B\)

\[B\to cSSSS\mid bSSS\mid aSS\mid dS\mid cSSSC'S\mid bSSC'S\mid aSC'S\mid dC'S\mid c\]

And similarly for \(A\) and \(S\)

\begin{align*}A&\to cSSSSS\mid bSSSS\mid aSSS\mid dSS\mid cSSSC'SS\mid bSSC'SS\mid aSC'SS\mid dC'SS\mid cS\mid b\\
S&\to cSSSSSS\mid bSSSSS\mid aSSSS\mid dSSS\mid cSSSC'SSS\mid bSSC'SSS\mid aSC'SSS\mid dC'SSS\mid cSS\mid bS\mid a\end{align*}

And finally for \(C'\)

\begin{align*}C'&\to cSSSSSSSSS\mid bSSSSSSSS\mid aSSSSSSS\mid dSSSSSS\mid cSSSC'SSSSSS\\&\mid bSSC'SSSSSS\mid aSC'SSSSSS\mid dC'SSSSSS\mid cSSSSS\mid bSSSS\\&\mid aSSSC'\mid cSSSSSSSSSC'\mid bSSSSSSSSC'\mid aSSSSSSSC'\mid dSSSSSSC'\mid cSSSC'SSSSSSC'\\&\mid bSSC'SSSSSSC'\mid aSC'SSSSSSC'\mid dC'SSSSSSC'\mid cSSSSSC'\mid bSSSSC'\mid aSSSC'\end{align*}

Consider similarly the example:

\begin{align*}
    S &\to AA\\
    A &\to BaA\mid a\\
    B &\to SBA\mid b
\end{align*}

Once again, there is no pre-processing to do. We see that \(B\) involves indirect left-recursion. Thus, we write 

\begin{align*}
    B &\to AABA\mid b\\
      &\to BaAABA\mid aABA\mid b
\end{align*}

This involves direct left-recursion, so we write

\begin{align*}
    B &\to aABA\mid b\mid aABAB'\mid bB'\\
    B' &\to aAABA\mid aAABAB'
\end{align*}

We then substitute the productions for \(B\) into \(A\)

\begin{align*}
    A &\to aABAaA\mid baA\mid aABAB'aA\mid bB'aA\mid a
\end{align*}

and finally substitute the productions for \(A\) into \(S\)

\begin{align*}
    S &\to aABAaAA\mid baAA\mid aABAB'aAA\mid bB'aAA\mid aA
\end{align*}

In total, our GNF is 

\begin{align*}
    S &\to aABAaAA\mid baAA\mid aABAB'aAA\mid bB'aAA\mid aA\\
    A &\to aABAaA\mid baA\mid aABAB'aA\mid bB'aA\mid a\\
    B &\to aABA\mid b\mid aABAB'\mid bB'\\
    B' &\to aAABA\mid aAABAB'
\end{align*}